\chapter{Introduction}
\citep{Kuijken_2008}, \cite{Refregier_2003_1}, \cite{Refregier_2003_2} \cite{Kuijken_2015}

\begin{equation}
    L_{lmn}(a,b,c) = \tfrac{1}{\sqrt{\pi}}\int dx\; e^{-x^2}H_l(ax)H_m(bx)H_n(cx)
\end{equation}

Using the explicit expression of the Hermite polynomial

\begin{align}
    H_n(ax)&=\sum_{m=0}^{\lfloor\frac{n}{2}\rfloor}\frac{n!(-1)^m}{m!(n-2m)!}(2ax)^{n-2m}\\&=\sum_{m=0}^{\lfloor\frac{n}{2}\rfloor}h_{m,n}(a)x^{n-2m}
\end{align}

with 

\begin{equation}
    h_{m,n}(a)=\frac{n!(-1)^m(2a)^{n-2m}}{m!(n-2m)!}
\end{equation}

we find

\begin{align}
    L_{lmn}(a,b,c) &= \tfrac{1}{\sqrt{\pi}}\int dx\; e^{-x^2}\sum_{i=0}^{\lfloor\frac{l}{2}\rfloor}h_{i,l}(a)x^{l-2i}\sum_{j=0}^{\lfloor\frac{m}{2}\rfloor}h_{j,m}(b)x^{m-2j}\sum_{k=0}^{\lfloor\frac{n}{2}\rfloor}h_{k,n}(c)x^{n-2k}\\
     &= \tfrac{1}{\sqrt{\pi}}\int dx\; e^{-x^2}\sum_{i=0}^{\lfloor\frac{l}{2}\rfloor}\sum_{j=0}^{\lfloor\frac{m}{2}\rfloor}\sum_{k=0}^{\lfloor\frac{n}{2}\rfloor}h_{i,l}(a)h_{j,m}(b)h_{k,n}(c)x^{l+m+n-2(i+j+k)}\\
     &= \tfrac{1}{\sqrt{\pi}}\sum_{i=0}^{\lfloor\frac{l}{2}\rfloor}\sum_{j=0}^{\lfloor\frac{m}{2}\rfloor}\sum_{k=0}^{\lfloor\frac{n}{2}\rfloor}h_{i,l}(a)h_{j,m}(b)h_{k,n}(c)\int dx\; e^{-x^2}x^{l+m+n-2(i+j+k)}
\end{align}

Using the fact that $L_{lmn}$ is only non-zero when $l+m+n$ is even, we can use

\begin{equation}
    \int dx\;x^{2n}e^{-x^2}=\sqrt{\pi}\frac{(2n)!}{n!}\left(\frac{1}{2}\right)^{2n}
\end{equation}

to evaluate the integral.

% \begin{align}
%     L_{lmn}(a,b,c) &= \sum_{i=0}^{\lfloor\frac{l}{2}\rfloor}\sum_{j=0}^{\lfloor\frac{m}{2}\rfloor}\sum_{k=0}^{\lfloor\frac{n}{2}\rfloor}h_{i,l}(a)h_{j,m}(b)h_{k,n}(c)\frac{(l+m+n-2(i+j+k))!}{((l+m+n)/2-(i+j+k)!}\left(\frac{1}{2}\right)^{l+m+n-2(i+j+k)}
% \end{align}

\begin{align}
L_{lmn}(a,b,c) &= 
\sum_{i=0}^{\lfloor\frac{l}{2}\rfloor}
\sum_{j=0}^{\lfloor\frac{m}{2}\rfloor}
\sum_{k=0}^{\lfloor\frac{n}{2}\rfloor}
h_{i,l}(a)\, h_{j,m}(b)\, h_{k,n}(c) \\
&\quad\;\, \times 
\frac{(l+m+n-2(i+j+k))!}
     { \left( \frac{l+m+n}{2} - (i+j+k) \right)! }
\left( \frac{1}{2} \right)^{\,l+m+n-2(i+j+k)}
\end{align}